\left(k \geq 10 , \left(m - 3\right) \geq \left(k + 1\right) , \left(k + l - 2\right) = \left(m + 4\right) , l \in \mathbb{N} , \left(l - 2\right) \in \mathbb{N} , m \in \mathbb{N} , \left(m - 4\right) \in \mathbb{N} , k \in \mathbb{N} , 10 \in \mathbb{N} , \left(10 + 1\right) = 11 , \forall_{i, j \in \mathbb{N}}~\left[\forall_{\bm{x}, \bm{y}}~\left(\left(\bm{x} \cdot \bm{y}\right) = \left(\left(\bm{x}_{i} \cdot \bm{y}_{i}\right) + \ldots + \left(\bm{x}_{j} \cdot \bm{y}_{j}\right)\right)\right)\right]\right)